\subsubsection*{Answer 1}
\textbf{(a)}
We need to find parameters \(w_1\), \(w_2\), and \(b\) such that the RNN generates the output sequence \([0, 0, 0, 1, 1, 1, 1]\) given the input sequence \([0, 0, 0, 1, 0, 1, 0]\).
The hidden state \(s_t\) is computed as:
$
s_t = \text{step}(w_1 x_t + w_2 s_{t-1} + b),
$
where \(\text{step}(z) = 1\) if \(z > 0\), and \(0\) otherwise. 
The output \(y_t = s_t\).

To generate the desired output sequence, we analyze the input and output transitions:
\begin{enumerate}
   \item Time step 1-3: Input is \(0\), output is \(0\). This implies:
   \[
   w_1 \cdot 0 + w_2 \cdot 0 + b \leq 0 \implies b \leq 0.
   \]

   \item Time step 4: Input is \(1\), output transitions to \(1\). This requires:
   \[
   w_1 \cdot 1 + w_2 \cdot 0 + b > 0 \implies w_1 + b > 0.
   \]

   \item Time step 5-7: Input alternates between \(0\) and \(1\), but output remains \(1\). This requires:
   \[
   w_1 \cdot x_t + w_2 \cdot 1 + b > 0 \quad \text{for all } x_t \in \{0, 1\}.
   \]
\end{enumerate}

To satisfy these conditions, we can set:
\[
w_1 = 1, \quad w_2 = 2, \quad b = -1.
\]

\textbf{Verification:}

   \begin{itemize}
      \item For \(t = 1-3\): \(s_t = \text{step}(1 \cdot 0 + 2 \cdot 0 - 1) = 0\).

      \item For \(t = 4\): \(s_4 = \text{step}(1 \cdot 1 + 2 \cdot 0 - 1) = \text{step}(0) = 1\).

      \item For \(t \geq 5\): \(s_t = \text{step}(1 \cdot x_t + 2 \cdot 1 - 1)\). Since \(x_t \geq 0\), \(1 \cdot x_t + 2 \cdot 1 - 1 \geq 1 > 0\), so \(s_t = 1\).
   \end{itemize}

\textbf{(b)} 
It is not possible to use the given RNN to generate the output sequence \([1, 1, 1, 0, 0, 0, 1, 1]\) from the input sequence \([0, 0, 0, 1, 0, 0, 1, 0]\). 
The output sequence starts with \(1\), which requires \(s_0 = 1\). However, the problem states \(s_0 = 0\), which is a contradiction.
Even if \(s_0 = 1\), the output sequence transitions from \(1\) to \(0\) at \(t=4\). This would require:
  \[
  w_1 \cdot x_4 + w_2 \cdot s_3 + b \leq 0.
  \]
  But \(x_4 = 1\) and \(s_3 = 1\), so:
  \[
  w_1 + w_2 + b \leq 0.
  \]
  However, the output transitions back to \(1\) at \(t=7\), requiring:
  \[
  w_1 \cdot x_7 + w_2 \cdot s_6 + b > 0.
  \]
  Since \(x_7 = 1\) and \(s_6 = 0\), this implies:
  \[
  w_1 + b > 0.
  \]
  These two conditions are contradictory:
  \[
  w_1 + w_2 + b \leq 0 \quad \text{and} \quad w_1 + b > 0.
  \]
  Therefore, no parameters \(w_1, w_2, b\) can satisfy both.
